progs/verif_insertion_sort.v
@@ -18,13 +18,16 @@ Fixpoint insert x xs :=
 
 Definition insert_spec :=
   DECLARE _insert
-    WITH sh: share, contents : list int, v : int
-    PRE [ _value OF tint, _sorted OF (tptr t_struct_list)]
+    WITH sh: share, contents : list int, insert_val : int, sorted : val
+    PRE [_insert_node OF (tptr t_struct_list), _sorted OF (tptr t_struct_list)]
         PROP ()
-        LOCAL (`(eq (Vint v)) (eval_id _value); `isptr (eval_id _sorted))
-        SEP (`(lseg LS sh contents) (eval_id _sorted) `nullval)
+        LOCAL (`eq (eval_id _sorted) `sorted)
+        SEP (`(lseg LS sh contents) (eval_id _sorted) `nullval;
+             `(list_cell LS sh) (eval_id _insert_node) `(insert_val);
+             `(field_mapsto sh t_struct_list _tail) (eval_id _insert_node) 
+                                                    `(nullval))
     POST [tptr t_struct_list]
-        `(lseg LS sh (insert v contents)) retval `nullval.
+        `(lseg LS sh (insert insert_val contents)) retval `nullval.
         
 Definition Vprog : varspecs := nil.
 
@@ -54,27 +57,29 @@ Definition fst_3 {A B C} (a: A* B*C) := fst (fst a).
 Definition snd_3 {A B C} (a: A * B * C) := snd (fst a).
 Definition third_3 {A B C} (a: A * B * C) := snd a.
 
-Definition insert_invariant sh value contents :=
+Definition insert_invariant sh insert_val contents :=
 EX contents_lt: list int,
 EX contents_rest : list int,
 EX sorted_val : int,
 EX next_ptr : val,
-PROP (Forall (Igt value) (contents_lt); 
+PROP (Forall (Igt insert_val) (contents_lt); 
       (contents_lt) ++ 
          (sorted_val)::(contents_rest) = contents)
-LOCAL ( `(eq (Vint value)) (eval_id _value);
+LOCAL ( `(eq (Vint insert_val)) (eval_id _insert_value);
         `(eq (Vint (sorted_val))) (eval_id _sortedvalue);
   `eq (eval_id _guard)
         (`logical_and_result `(tptr t_struct_list) 
            (eval_id _index) `tint
-           (`(eval_binop Ogt tint tint) (eval_id _value)
+           (`(eval_binop Ogt tint tint) (eval_id _insert_value)
              (eval_id _sortedvalue))))
 SEP (`(lseg LS sh (contents_lt)) (eval_id _sorted) (eval_id _index);
      `(list_cell LS sh) (eval_id _index) `(sorted_val);
-      `(field_mapsto sh t_struct_list _tail) (eval_id _index) 
+     `(field_mapsto sh t_struct_list _tail) (eval_id _index) 
                            `(next_ptr);
-      `(lseg LS sh (contents_rest)) `(next_ptr) `nullval;
-      (var_block Tsh (_newitem, t_struct_list))).
+     `(lseg LS sh (contents_rest)) `(next_ptr) `nullval;
+     `(list_cell LS sh) (eval_id _insert_node) `(insert_val);
+     `(field_mapsto sh t_struct_list _tail) (eval_id _insert_node) 
+                         `(nullval)).
 
 Lemma lseg_cons_non_nill : forall {ls ll} LS sh h r v1 v2 , @lseg ls ll LS sh (h::r) v1 v2 = 
 !!isptr v1 && @lseg ls ll LS sh (h::r) v1 v2.
@@ -105,33 +110,110 @@ apply IHl1. intuition.
 inv H0; auto.
 Qed.
 
+Lemma lseg_is_ptr_or_null : 
+forall {ls ll} LS sh c v1 v2 R, 
+@lseg ls ll LS sh (c) v1 v2 * R |-- !!is_pointer_or_null v1 && (@lseg ls ll LS sh c v1 v2)  * R.
+Proof.
+intros.
+cancel.
+normalize.
+apply andp_right.
+rewrite lseg_unroll. 
+apply orp_left. rewrite andp_assoc.
+Admitted. (* fix by changing ptr_eq once things are more stable*)
+
 Lemma body_insert: semax_body Vprog Gtot f_insert insert_spec.
 Proof.
 start_function.
-name value _value.
+name insert_value _insert_value.
 name index _index.
-name sorted _sorted.
-forward. (*  index = sorted; *)
-focus_SEP 1.
-apply semax_lseg_nonnull.
-go_lower. normalize. intros first_val tail_vals tail_ptr ?.
+name insert_node _insert_node.
+name sortv _sorted.
 rewrite lift_list_cell_eq.
-forward. (*sortedvalue = index -> head;*)
+forward. (*insert_value = insert_node -> head;*)
+forward. (*index = sorted; *)
+forward_if
+(EX first_val : int,
+ EX tail_vals : list int,
+ EX tail_ptr : val,
+PROP  ()
+      LOCAL 
+      (`eq (eval_id _index)
+         (eval_expr (Etempvar _sorted (tptr t_struct_list)));
+      `(eq (Vint insert_val)) (eval_id _insert_value);
+      (if(isptrb sorted) then 
+         `(eq (Vint first_val)) (eval_id _sortedvalue)
+       else
+         `True))
+      SEP  (
+       if(isptrb sorted) then
+         `(field_mapsto sh t_struct_list _head) (eval_id _sorted) 
+            `(Vint first_val) *
+         `(field_mapsto sh t_struct_list _tail) (eval_id _sorted) `tail_ptr *
+         `(lseg LS sh tail_vals) `tail_ptr `nullval
+         else
+          `(lseg LS sh tail_vals nullval nullval);
+      `(field_mapsto sh t_struct_list _head) (eval_id _insert_node)
+        (`Vint `insert_val);
+      `(field_mapsto sh t_struct_list _tail) (eval_id _insert_node) `nullval)).
+entailer.
+apply semax_lseg_nonnull.
+go_lower. subst. normalize.
+intros first_val tail_vals tail_ptr ?.
+
+(*sortedvalue = index -> head;*)
+{ rewrite lift_list_cell_eq.
+  apply sequential'.
+  hoist_later_in_pre.
+  eapply semax_post_flipped.
+  eapply (semax_load_field_37); try reflexivity.
+  go_lower. apply prop_right; auto.
+  entailer!.
+  intros. apply andp_left2.
+  apply normal_ret_assert_derives'.
+  entailer.
+  apply (exp_right first_val).
+  apply (exp_right tail_vals).
+  apply (exp_right tail_ptr).
+  autorewrite with subst.
+  entailer.
+  rewrite H2 in *.
+  destruct (eval_id _sorted rho); inv H4.
+  simpl.
+  entailer.
+  rewrite H in *.
+  cancel.
+  cancel. eapply lseg_unroll_nonempty1.
+  auto. apply H5. cancel.
+}
+{
+  apply sequential'.
+  eapply semax_post_flipped.
+  eapply semax_skip.
+  intros.
+  apply andp_left2.
+  apply normal_ret_assert_derives'.
+  go_lower.
+  subst.
+  rewrite H0 in *.
+  rewrite H. simpl.
+  entailer!.
+}
+abbreviate_semax.
 forward. (*guard' = index && (value > sortedvalue);*) 
-  
+admit.   (* need closed lemma *)
+entailer. apply prop_right; split; auto.
+
+unfold denote_tc_initialized. simpl Map.get.
 forward. (*guard = guard'*) 
 simpl typeof.
 {
-
-
-
-
-
-
 forward_while (insert_invariant sh v contents) (insert_invariant sh v contents).
 (*pre implies invariant*)
-unfold insert_invariant. apply (exp_right (nil, tail_vals)). 
-eapply (exp_right (first_val,tail_ptr)). 
+apply (exp_right nil).
+apply (exp_right tail_vals).
+apply (exp_right first_val).
+apply (exp_right tail_ptr).
 entailer.
 { apply andp_right. 
   + rewrite H1. apply prop_right. rewrite <- H3 in *. auto. 
@@ -140,16 +222,14 @@ entailer.
 (*guard typechecks*)
 entailer.
 (*invariant implies post *)
-unfold insert_invariant.
-apply (exp_right all_contents). 
-apply (exp_right sorted_val__next_ptr).
+apply (exp_right contents_lt).
+apply (exp_right contents_rest).
+apply (exp_right sorted_val).
+apply (exp_right next_ptr).
 entailer.
 (*invariant across command *) 
 forward. 
 (* unfold the remaining part of the list *)
-destruct sorted_val__next_ptr as [sorted_val next_ptr]. 
-destruct all_contents as [contents_lt contents_rest]. 
-unfold fst, snd.
 forward. (*    index = index -> tail; *)
 (* if(index) *)
 forward_if 
@@ -221,6 +301,7 @@ entailer.
 (*needs work, most of this should be in forward *)
 (*sortedvalue = index -> head;*)
 { rewrite lift_list_cell_eq.
+  new_load_tac.
   apply sequential'.
   hoist_later_in_pre.
   eapply semax_post_flipped.
@@ -269,17 +350,17 @@ apply extract_exists_pre; intro index_ptr2.
 apply extract_exists_pre; intro rest_index_vals2.
 apply extract_exists_pre; intro old_sortedvalue.
 forward.
-admit. (* fix this*)
+admit.
 admit.
 forward.
+
 (*implies post*)
-unfold insert_invariant.
-unfold loop1_ret_assert.
-unfold subst, fst_3, snd_3, fst, snd in *.
 remember (isptrb next_ptr).
 { destruct b.
-  + apply (exp_right (contents_lt ++ sorted_val :: [], rest_index_vals2)).
-    apply (exp_right (index_val2, index_ptr2)).
+  + apply (exp_right (contents_lt ++ sorted_val :: nil)).
+    apply (exp_right (rest_index_vals2)).
+    apply (exp_right (index_val2)).
+    apply (exp_right index_ptr2).
     entailer.
     rewrite <- H4 in *.
     apply andp_right.
@@ -288,21 +369,24 @@ remember (isptrb next_ptr).
          auto.
          simpl in H5.
          simpl in H8.
-         clear - H8 H7.
-         destruct (eval_id _previous rho); inv H7.
+         clear - H8 H.
+         destruct (eval_id _previous rho); inv H.
          unfold logical_and_result in *.
          simpl in *. constructor. unfold Igt.
          replace (Int.lt sorted_val value) with
            (Int.cmp Clt sorted_val value) in * by auto.
          SearchAbout Int.cmp.
          remember (Int.cmp Clt sorted_val value).
-         destruct b0; inv H8. SearchAbout Int.cmp.
+         destruct b0; inv H8. 
          rewrite <- Int.swap_cmp in Heqb0. simpl swap_comparison in Heqb0.
          auto. auto. 
          split. 
          rewrite app_assoc_reverse. simpl. auto. 
          auto.
-       - cancel. admit. (*seems reasonable *)
+       - unfold subst. cancel.
+         autorewrite with subst.
+         cancel. 
+         admit. (*seems reasonable *)
   + apply (exp_right (contents_lt , nil)).
     apply (exp_right (sorted_val, nullval)).
     entailer.
